tDag.thy
@@ -1,0 +1,80 @@
+theory tDag
+imports rBox
+begin
+
+(*Datentyp trapez und directed acyclic graph(dag)-struktur für Trapeze*)
+
+(*Defintion für trapez. durch Strecke über dem Trapez, Strecke unter dem Trapez.
+linker Endpunkt, rechter Endpunkt*)
+typedef trapez = "{p::((point2d*point2d)*(point2d*point2d)*point2d*point2d). True}" by(auto)
+definition topT :: "trapez \<Rightarrow> (point2d\<times>point2d)" where  "topT T \<equiv> fst(Rep_trapez T)"
+definition bottomT :: "trapez \<Rightarrow> (point2d\<times>point2d)" where "bottomT T \<equiv> fst(snd(Rep_trapez T))"
+definition leftP :: "trapez \<Rightarrow> point2d" where "leftP T \<equiv> fst(snd(snd(Rep_trapez T)))"
+definition rightP :: "trapez \<Rightarrow> point2d" where "rightP T \<equiv> snd(snd(snd(Rep_trapez T)))"
+lemma topTSimp [simp] : "topT (Abs_trapez ((a,b),(c,d),e,f)) = (a,b)" by (simp add: topT_def Abs_trapez_inverse)
+lemma bottomTSimp [simp] : "bottomT (Abs_trapez ((a,b),(c,d),e,f)) = (c,d) "by (simp add: bottomT_def Abs_trapez_inverse)
+lemma leftPSimp [simp] : "leftP (Abs_trapez ((a,b),(c,d),e,f)) = e" by (simp add: leftP_def Abs_trapez_inverse)
+lemma rightPSimp [simp] : "rightP (Abs_trapez ((a,b),(c,d),e,f)) = f" by (simp add: rightP_def Abs_trapez_inverse)
+lemma trapezSameCoord [simp]: "(Abs_trapez ((a,b),(c,d),e,f) = Abs_trapez ((a',b'),(c',d'),e',f'))
+  \<longleftrightarrow> a=a'\<and> b=b' \<and> c=c' \<and> d=d' \<and> e=e' \<and> f=f'"
+  by (metis Abs_trapez_inverse Collect_const UNIV_I fst_conv snd_conv)
+
+
+(*ein Trapez und seine Nachbarn*)
+(*record trapezoid = trapez :: trapez
+  upRightNeighbor :: "trapez"
+  lowerRightNeighbor :: "trapez"
+  upLeftNeighbor :: "trapez"
+  lowerLeftNeighbor :: "trapez"*)
+
+(*Knoten des graphen kann enweder ein Endpunkt sein, oder ein Segment*)
+datatype_new kNode = xNode "point2d" | yNode "(point2d\<times>point2d)"
+
+(*directed acyclic graph*)
+(*x-nodes stores a segment endpoint that defines a vertical extension in the trapezoid map,
+and has leftChild() and rightChild() pointers to nodes.*)
+(*y-node stores a line segment and its children are also recorded by the pointers are aboveChild()
+and belowChild() depending on whether the child item is above or below the segment stored at the y-node.*)
+datatype_new dag = Tip "trapez" | Node "dag" kNode "dag"
+
+(*wann ist ein Trapez im Baum*)
+fun tipInDag :: "trapez \<Rightarrow> dag \<Rightarrow> bool" where
+  "tipInDag T (Tip D) = (if (T = D) then True else False)"
+  | "tipInDag T (Node Tl x Tr) = (tipInDag T Tl \<or> tipInDag T Tr)"
+
+(*Input Tip welches entfernt wird, dag welches hinzugefügt wird, dag-tree in dem ersetzt werden soll
+Output: neues dag-tree*)
+fun replaceTip :: "trapez \<Rightarrow> dag \<Rightarrow> dag \<Rightarrow> dag" where
+  "replaceTip oT nT (Tip D) = (if (D = oT) then (nT) else (Tip D))"
+ |"replaceTip oT nT (Node Tl x Tr) = Node (replaceTip oT nT Tl) x (replaceTip oT nT Tr)"
+
+lemma replaceMiss [simp]: "\<not>tipInDag oT D \<Longrightarrow> replaceTip oT nT D = D"
+  by (induction oT nT D rule: replaceTip.induct, case_tac "oT = D", simp+)
+lemma replaceMiss1: "\<not>tipInDag oT D \<Longrightarrow> \<not>tipInDag oT (replaceTip oT nT D)"
+  by (induction oT nT D rule: replaceTip.induct, case_tac "oT = D", simp+)
+
+lemma replaceTipSize1 : "size (replaceTip oT (Tip nT) D) = size D"
+  by (induction oT "Tip nT" D rule: replaceTip.induct, simp+)
+lemma replaceTipSize : "size (replaceTip oT nT D) \<ge> size D"
+  by (induction oT nT D rule: replaceTip.induct, simp+)
+
+lemma replaceTipSame [simp] : "replaceTip oT (Tip oT) D = D"
+  by (induction oT "(Tip oT)" D rule: replaceTip.induct, simp+)
+
+lemma "nT\<noteq>D\<Longrightarrow> replaceTip oT nT D = replaceTip oT D nT \<Longrightarrow> False"
+  apply (induction D, simp)
+  apply (case_tac "x = oT")
+oops
+theorem "\<not>tipInDag nT' D \<Longrightarrow> replaceTip nT' nT (replaceTip oT (Tip nT') D) = replaceTip oT nT D"
+  apply (induction D, case_tac "nT' = x", simp+)
+done
+theorem "replaceTip oT nT (replaceTip oT' nT' D) = replaceTip oT' nT' (replaceTip oT nT D) \<Longrightarrow> False"
+  apply (induction oT nT D rule: replaceTip.induct)
+  apply (simp)
+  apply (case_tac "oT'= oT")
+  apply (case_tac "D = oT'")
+  apply (simp)
+oops
+
+
+end
